cfrontend/BeePL_proof.v
@@ -2,7 +2,7 @@ Require Import String ZArith Coq.FSets.FMapAVL Coq.Structures.OrderedTypeEx.
 Require Import Coq.FSets.FSetProperties Coq.FSets.FMapFacts FMaps FSetAVL Nat PeanoNat.
 Require Import Coq.Arith.EqNat Coq.ZArith.Int Integers AST Maps Linking Ctypes Smallstep SimplExpr.
 Require Import BeePL_aux BeePL_mem BeeTypes BeePL Csyntax Clight Globalenvs BeePL_Csyntax SimplExpr.
-Require Import compcert.common.Errors Initializersproof Cstrategy BeePL_auxlemmas lib.Coqlib.
+Require Import compcert.common.Errors Initializersproof Cstrategy BeePL_auxlemmas lib.Coqlib Errors.
 
 From mathcomp Require Import all_ssreflect. 
 
@@ -132,11 +132,10 @@ Admitted.
 Section specifications.
 
 (* Relates global variables of BeePL and Csyntax *)
-Inductive match_globvar : BeePL.globvar -> AST.globvar Ctypes.type -> Prop :=
+Inductive match_globvar : BeePL.globvar type -> AST.globvar Ctypes.type -> Prop :=
 | match_globvar_intro : forall t init t' init' rd vo,
   transBeePL_type t = OK t' ->
   rel_type t t' ->
-  transBeePL_init_datas_init_datas init = init' ->
   match_globvar (mkglobvar t init rd vo) (AST.mkglobvar t' init' rd vo).
 
 (* Relates the function definition of BeePL and Csyntax *)
@@ -154,15 +153,15 @@ Inductive match_fundef : BeePL.fundef -> Csyntax.fundef -> Prop :=
   match_fundef (Internal f) (Ctypes.Internal cf).
 
 (* Relates the global definitions of BeePL and Csyntax *) 
-Inductive match_globdef : BeePL.globdef -> AST.globdef Csyntax.fundef Ctypes.type -> Prop :=
+Inductive match_globdef : BeePL.globdef BeePL.fundef type -> AST.globdef Csyntax.fundef Ctypes.type -> Prop :=
 | match_gfun : forall f cf,
   match_fundef f cf ->
-  match_globdef (Gfun f) (AST.Gfun cf)
+  match_globdef (AST.Gfun f) (AST.Gfun cf)
 | match_gvar : forall g cg,
   match_globvar g cg ->
   match_globdef (Gvar g) (AST.Gvar cg).
 
-Definition match_ident_globdef (igd1 : ident * BeePL.globdef) 
+Definition match_ident_globdef (igd1 : ident * BeePL.globdef BeePL.fundef type) 
   (igd2 : ident *  AST.globdef Csyntax.fundef Ctypes.type) : Prop :=
 fst igd1 = fst igd2 /\ match_globdef (snd igd1) (snd igd2).
 
@@ -171,14 +170,45 @@ Definition match_program_gen (p1 : BeePL.program) (p2 : Csyntax.program) : Prop 
   /\ p2.(AST.prog_main) = p1.(prog_main)
   /\ p2.(AST.prog_public) = p1.(prog_public).
 
+Definition match_prog (p1: BeePL.program) (p2: Csyntax.program) :=
+    match_program_gen p1 p2
+ /\ prog_types p1 = Ctypes.prog_types p2. 
+
+Lemma transf_program_match:
+forall p cp, BeePL_compcert p = OK cp -> match_prog p cp.
+Proof.
+rewrite /BeePL_compcert /=. move=> p cp H. monadInv H.
+split; auto; rewrite /match_program_gen /=; split; auto.
+move: x EQ. elim: (prog_defs p)=> //=.
+(* nil *)
++ move=> xs [] eq /=; subst. by apply list_forall2_nil.
+(* cons *)
+move=> [] id gd gds ih /= xs h. monadInv h.
+move: (ih x0 EQ1)=> hl. apply list_forall2_cons; auto.
+rewrite /match_ident_globdef /=; split; auto.
+rewrite /transBeePL_globdef_globdef in EQ. case: gd EQ=> //=.
++ move=> fd h. monadInv h. apply match_gfun. rewrite /transBeePL_fundef_fundef in EQ.
+  case: fd EQ=> //= f h. monadInv h. apply match_fundef_internal.
+  by rewrite /transBeePL_fundef_fundef /= EQ /=.
+move=> gv h. monadInv h. apply match_gvar. case: gv EQ=> //= gi i r v.
+case: x1=> //= gi' i' r' v'. rewrite /transBeePLglobvar_globvar /=. move=> h.
+monadInv h. apply match_globvar_intro; auto.
+have [h1 h2] := type_translated. by move: (h1 gi gi' EQ).
+Qed.
 
 End specifications.
 
 Section semantic_preservation.
 
-Variable beePLprog : BeePL.program.
+Variable bprog : BeePL.program.
 
 Variable cprog : Csyntax.program.
+
+Hypothesis TRANSBPL: match_prog bprog cprog.
+
+Let bge := Genv.globalenv (trans_program_astprog bprog).
+
+Let cge := Genv.globalenv cprog.
 
 End semantic_preservation.
 
